CaseStudy/Names.v
@@ -1,9 +1,7 @@
-Require Import List.
-Require Import FunctionalExtensionality.
+Require Import Coq.Lists.List.
+Require Import Coq.Logic.FunctionalExtensionality.
 Require Import Coq.Program.Equality.
-Require Import GDTC.Polynomial.
-Require Import GDTC.Containers.
-Require Import GDTC.Functors.
+Require Import GDTC.
 
 Section Names.
 
@@ -56,10 +54,10 @@ Section Names.
 
   (** ERROR VALUES **)
 
-   Inductive StuckValue (A : Set) : Set :=
-    | Stuck : nat -> StuckValue A.
+  Inductive StuckValue (A : Set) : Set :=
+  | Stuck : nat -> StuckValue A.
 
-   Context {Sub_StuckValue_V : StuckValue :<: V}.
+  Context {Sub_StuckValue_V : StuckValue :<: V}.
 
   Global Instance StuckValue_Container : Container StuckValue.
     apply (ConstContainer nat StuckValue
@@ -92,9 +90,7 @@ Section Names.
   Global Instance BotValue_Container : Container BotValue.
     apply (ConstContainer unit BotValue
             (fun A x => match x with Bot => tt end)
-            (fun A x => Bot _)).
-    destruct x; reflexivity.
-    destruct x; reflexivity.
+            (fun A x => Bot _)); destruct x; reflexivity.
   Defined.
 
   Context {Sub_BotValue_V : BotValue :<: V}.
@@ -103,7 +99,6 @@ Section Names.
   Context {WF_SubBotValue_V : WF_Functor _ _ Sub_BotValue_V}.
 
   Definition bot : Value := inject BotValue V (Bot _).
-  Hint Unfold bot.
 
   Definition ind_alg_Bot (P : Value -> Prop) (H : P bot) :
     PAlgebra (inject BotValue V) P :=
@@ -137,7 +132,7 @@ Section Names.
   Context {Fun_E : Functor E}.
   Context {PFun_E : PFunctor E}.
   Context {spf_E : SPF E}.
-  Definition Exp := Fix E.
+  Let Exp := Fix E.
 
   (* ============================================== *)
   (* OPERATIONS                                     *)
@@ -200,282 +195,292 @@ Section Names.
   Definition ValuePrint := fold_ (f_algebra ValuePrintName id).
 
   (* Printers for Bot and Stuck *)
-   Global Instance MAlgebra_ValuePrint_BotValue T : FAlgebra ValuePrintName T ValuePrintR BotValue :=
-     {| f_algebra :=  fun _ _ => append "bot" "" |}.
+  Global Instance MAlgebra_ValuePrint_BotValue T :
+    FAlgebra ValuePrintName T ValuePrintR BotValue :=
+    {| f_algebra :=  fun _ _ => append "bot" "" |}.
 
-   Global Instance MAlgebra_ValuePrint_StuckValue T : FAlgebra ValuePrintName T ValuePrintR StuckValue :=
-     {| f_algebra :=
-       fun _ e => match e with
-                      | Stuck n => append "Stuck " (String (ascii_of_nat (n + 48)) EmptyString)
-                    end|}.
+  Global Instance MAlgebra_ValuePrint_StuckValue T :
+    FAlgebra ValuePrintName T ValuePrintR StuckValue :=
+    {| f_algebra := fun _ e =>
+         match e with
+           | Stuck n =>
+             append "Stuck "
+                    (String (ascii_of_nat (n + 48)) EmptyString)
+         end
+    |}.
 
   (* ============================================== *)
   (* PREDICATE LIFTERS FOR LISTS                    *)
   (* ============================================== *)
 
-    (* Unary Predicates.*)
-    Inductive P_Env {A : Set} (P : A -> Prop) : forall (env : Env A), Prop :=
-    | P_Nil : P_Env P nil
-    | P_Cons : forall a (As : Env _), P a -> P_Env P As ->
-      P_Env P (cons a As).
+  (* Unary Predicates.*)
+  Inductive P_Env {A : Set} (P : A -> Prop) : forall (env : Env A), Prop :=
+  | P_Nil : P_Env P nil
+  | P_Cons a (As : Env _) : P a -> P_Env P As -> P_Env P (cons a As).
 
-    Lemma P_Env_lookup : forall A (env : Env A) P,
-      P_Env P env ->
-      forall n v,
-        lookup env n = Some v -> P v.
-      intros A env P P_env; induction P_env;
-        destruct n; simpl; intros; try discriminate.
-      injection H0; intros; subst; eauto.
-      eauto.
-    Qed.
+  Lemma P_Env_lookup A (env : Env A) P :
+    P_Env P env ->
+    forall n v,
+      lookup env n = Some v -> P v.
+  Proof.
+    intros P_env; induction P_env;
+    destruct n; simpl; intros; try discriminate.
+    injection H0; intros; subst; eauto.
+    eauto.
+  Qed.
 
-    Lemma P_Env_Lookup : forall A (env : Env A) (P : A -> Prop),
-      (forall n v,
-        lookup env n = Some v -> P v) ->
-      P_Env P env.
-      intros A env P H; induction env; constructor.
-      eapply (H 0); eauto.
-      apply IHenv; intros; eapply (H (S n)); eauto.
-    Qed.
+  Lemma P_Env_Lookup A (env : Env A) (P : A -> Prop) :
+    (forall n v,
+       lookup env n = Some v -> P v) ->
+    P_Env P env.
+  Proof.
+    intros H; induction env; constructor.
+    eapply (H 0); eauto.
+    apply IHenv; intros; eapply (H (S n)); eauto.
+  Qed.
 
-    Lemma P_Env_insert : forall A (env : Env A) (P : A -> Prop),
-      P_Env P env -> forall a, P a -> P_Env P (insert _ a env).
-      induction env; simpl; intros; constructor; eauto.
-      inversion H; subst; eauto.
-      eapply IHenv; inversion H; eauto.
-    Qed.
+  Lemma P_Env_insert A (env : Env A) (P : A -> Prop) :
+    P_Env P env -> forall a, P a -> P_Env P (insert _ a env).
+  Proof.
+    induction env; simpl; intros; constructor; eauto.
+    inversion H; subst; eauto.
+    eapply IHenv; inversion H; eauto.
+  Qed.
 
-    (* Binary Predicates.*)
-    Inductive P2_Env {A B : Set} (P : A -> B -> Prop) : forall (env : Env A) (env : Env B), Prop :=
-    | P2_Nil : P2_Env P nil nil
-    | P2_Cons : forall a b (As : Env _) (Bs : Env _), P a b -> P2_Env P As Bs ->
+  (* Binary Predicates.*)
+  Inductive P2_Env {A B : Set} (P : A -> B -> Prop) : forall (env : Env A) (env : Env B), Prop :=
+  | P2_Nil : P2_Env P nil nil
+  | P2_Cons a b (As : Env _) (Bs : Env _) :
+      P a b -> P2_Env P As Bs ->
       P2_Env P (cons a As) (cons b Bs).
 
-    Inductive P2_Shape {A B : Set} : Env A -> Env B -> Prop :=
-    | P2S_Nil : P2_Shape nil nil
-    | P2S_Cons : forall a b {As : Env _} {Bs : Env _}, P2_Shape As Bs ->
-      P2_Shape (cons a As) (cons b Bs).
+  Inductive P2_Shape {A B : Set} : Env A -> Env B -> Prop :=
+  | P2S_Nil : P2_Shape nil nil
+  | P2S_Cons : forall a b {As : Env _} {Bs : Env _}, P2_Shape As Bs ->
+    P2_Shape (cons a As) (cons b Bs).
 
-    Fixpoint P2_Shape_irrelevance {A B : Set} {As : Env A} {Bs : Env B}
-             (s : P2_Shape As Bs) : forall s', s = s'.
-    Proof.
-      destruct s.
-      intros s'.
-      dependent destruction s'.
-      reflexivity.
-      intros s'.
-      dependent destruction s'.
-      rewrite (P2_Shape_irrelevance A B As Bs s s').
-      reflexivity.
-    Defined.
+  Fixpoint P2_Shape_irrelevance {A B : Set} {As : Env A} {Bs : Env B}
+           (s : P2_Shape As Bs) : forall s', s = s'.
+  Proof.
+    destruct s.
+    intros s'.
+    dependent destruction s'.
+    reflexivity.
+    intros s'.
+    dependent destruction s'.
+    rewrite (P2_Shape_irrelevance A B As Bs s s').
+    reflexivity.
+  Qed.
 
-    Definition P2_Env_Shape {A B : Set} {P : A -> B -> Prop} {As : Env A} {Bs : Env B} :
-      P2_Env P As Bs -> P2_Shape As Bs.
-    Proof.
-      intros ps; induction ps; constructor; auto.
-    Defined.
+  Definition P2_Env_Shape {A B : Set} {P : A -> B -> Prop} {As : Env A} {Bs : Env B} :
+    P2_Env P As Bs -> P2_Shape As Bs.
+  Proof.
+    intros ps; induction ps; constructor; auto.
+  Defined.
 
-    Inductive P2_Index {A B : Set} (a : A) (b : B) :
-      forall {As : Env A} {Bs : Env B}, P2_Shape As Bs -> Set :=
-    | P2I_Here  : forall {As Bs} (s : P2_Shape As Bs),
-                    P2_Index a b (P2S_Cons a b s)
-    | P2I_There : forall a' b' {As Bs} (s : P2_Shape As Bs),
-                    P2_Index a b s ->
-                    P2_Index a b (P2S_Cons a' b' s).
+  Inductive P2_Index {A B : Set} (a : A) (b : B) :
+    forall {As : Env A} {Bs : Env B}, P2_Shape As Bs -> Set :=
+  | P2I_Here  : forall {As Bs} (s : P2_Shape As Bs),
+      P2_Index a b (P2S_Cons a b s)
+  | P2I_There : forall a' b' {As Bs} (s : P2_Shape As Bs),
+      P2_Index a b s ->
+      P2_Index a b (P2S_Cons a' b' s).
 
-    Fixpoint P2_tabulate {A B : Set} {P : A -> B -> Prop}
-      {As : Env A} {Bs : Env B} (s : P2_Shape As Bs) :
+  Fixpoint P2_tabulate {A B : Set} {P : A -> B -> Prop}
+    {As : Env A} {Bs : Env B} (s : P2_Shape As Bs) :
       (forall (a : A) (b : B), P2_Index a b s -> P a b) -> P2_Env P As Bs :=
-      match s in (P2_Shape As Bs) return
-        ((forall a b, P2_Index a b s -> P a b) -> P2_Env P As Bs)
-      with
-        | P2S_Nil => fun _ => P2_Nil P
-        | P2S_Cons _ _ _ _ s =>
-          fun pf =>
-            P2_Cons _ _ _ _ _
-              (pf _ _ (P2I_Here _ _ s))
-              (P2_tabulate _
-                 (fun _ _ i => pf _ _ (P2I_There _ _ _ _ s i)))
-      end.
+    match s in (P2_Shape As Bs) return
+      ((forall a b, P2_Index a b s -> P a b) -> P2_Env P As Bs)
+    with
+      | P2S_Nil => fun _ => P2_Nil P
+      | P2S_Cons _ _ _ _ s =>
+        fun pf =>
+          P2_Cons _ _ _ _ _
+            (pf _ _ (P2I_Here _ _ s))
+            (P2_tabulate _
+               (fun _ _ i => pf _ _ (P2I_There _ _ _ _ s i)))
+    end.
 
-    Fixpoint P2_lookup {A B : Set} {P : A -> B -> Prop}
-      {As : Env A} {Bs : Env B} (s : P2_Shape As Bs) (ps : P2_Env P As Bs) :
+  Fixpoint P2_lookup {A B : Set} {P : A -> B -> Prop}
+    {As : Env A} {Bs : Env B} (s : P2_Shape As Bs) (ps : P2_Env P As Bs) :
       forall (a : A) (b : B), P2_Index a b s -> P a b.
-    Proof.
-      intros a b idx.
-      destruct idx.
-      inversion ps.
-      apply H2.
-      inversion ps.
-      apply (P2_lookup _ _ _ _ _ _ H4 _ _ idx).
-    Defined.
+  Proof.
+    intros a b idx.
+    destruct idx.
+    inversion ps.
+    apply H2.
+    inversion ps.
+    apply (P2_lookup _ _ _ _ _ _ H4 _ _ idx).
+  Defined.
 
-    Fixpoint P2_tabulate_lookup' {A B : Set} {P : A -> B -> Prop}
-             {As : Env A} {Bs : Env B}
-             (ps : P2_Env P As Bs) :
+  Fixpoint P2_tabulate_lookup' {A B : Set} {P : A -> B -> Prop}
+    {As : Env A} {Bs : Env B}
+    (ps : P2_Env P As Bs) :
       P2_tabulate (P2_Env_Shape ps) (P2_lookup (P2_Env_Shape ps) ps) = ps.
-    Proof.
-      destruct ps; simpl.
-      reflexivity.
-      simpl.
-      f_equal.
-      apply (P2_tabulate_lookup' A B P As Bs ps).
-    Qed.
+  Proof.
+    destruct ps; simpl.
+    reflexivity.
+    simpl.
+    f_equal.
+    apply (P2_tabulate_lookup' A B P As Bs ps).
+  Qed.
 
-    Lemma P2_tabulate_lookup {A B : Set} {P : A -> B -> Prop}
-             {As : Env A} {Bs : Env B}
-             (ps : P2_Env P As Bs)
-    : forall s, P2_tabulate s (P2_lookup s ps) = ps.
-    Proof.
-      intro s.
-      rewrite (P2_Shape_irrelevance s (P2_Env_Shape ps)).
-      apply P2_tabulate_lookup'.
-    Qed.
+  Lemma P2_tabulate_lookup {A B : Set} {P : A -> B -> Prop}
+    {As : Env A} {Bs : Env B}
+    (ps : P2_Env P As Bs) :
+      forall s, P2_tabulate s (P2_lookup s ps) = ps.
+  Proof.
+    intro s.
+    rewrite (P2_Shape_irrelevance s (P2_Env_Shape ps)).
+    apply P2_tabulate_lookup'.
+  Qed.
 
-    Lemma P2_lookup_tabulate {A B : Set} (P : A -> B -> Prop)
-             {As : Env A} {Bs : Env B} (s : P2_Shape As Bs)
-             (f : forall (a : A) (b : B), P2_Index a b s -> P a b)
-             (a : A) (b : B) (i : P2_Index a b s)
-    : P2_lookup s (P2_tabulate s f) _ _ i = f _ _ i.
-    Proof.
-      induction i; simpl.
-      reflexivity.
-      rewrite IHi.
-      reflexivity.
-    Qed.
+  Lemma P2_lookup_tabulate {A B : Set} (P : A -> B -> Prop)
+    {As : Env A} {Bs : Env B} (s : P2_Shape As Bs)
+    (f : forall (a : A) (b : B), P2_Index a b s -> P a b)
+    (a : A) (b : B) (i : P2_Index a b s) :
+      P2_lookup s (P2_tabulate s f) _ _ i = f _ _ i.
+  Proof.
+    induction i; simpl.
+    reflexivity.
+    rewrite IHi.
+    reflexivity.
+  Qed.
 
-    Lemma P2_Env_lookup : forall A B (env : Env A) (env' : Env B) P,
-      P2_Env P env env' ->
-      forall n v,
-        lookup env n = Some v -> exists v', lookup env' n = Some v' /\
-          P v v'.
-      intros A B env env' P P_env_env'; induction P_env_env';
-        destruct n; simpl; intros; try discriminate.
-      exists b; injection H0; intros; subst; split; eauto.
-      eauto.
-    Qed.
+  Lemma P2_Env_lookup A B (env : Env A) (env' : Env B) P :
+    P2_Env P env env' ->
+    forall n v,
+      lookup env n = Some v -> exists v', lookup env' n = Some v' /\ P v v'.
+  Proof.
+    intros P_env_env'; induction P_env_env';
+      destruct n; simpl; intros; try discriminate.
+    exists b; injection H0; intros; subst; split; eauto.
+    eauto.
+  Qed.
 
-    Lemma P2_Env_lookup' : forall A B (env : Env A) (env' : Env B) P,
-      P2_Env P env env' ->
-      forall n v,
-        lookup env' n = Some v -> exists v', lookup env n = Some v' /\
-          P v' v.
-      intros A B env env' P P_env_env'; induction P_env_env';
-        destruct n; simpl; intros; try discriminate.
-      eexists; injection H0; intros; subst; split; eauto.
-      eauto.
-    Qed.
+  Lemma P2_Env_lookup' A B (env : Env A) (env' : Env B) P :
+    P2_Env P env env' ->
+    forall n v,
+      lookup env' n = Some v ->
+      exists v', lookup env n = Some v' /\ P v' v.
+  Proof.
+    intros P_env_env'; induction P_env_env';
+      destruct n; simpl; intros; try discriminate.
+    eexists; injection H0; intros; subst; split; eauto.
+    eauto.
+  Qed.
 
-    Lemma P2_Env_Nlookup : forall A B (env : Env A) (env' : Env B) P,
-      P2_Env P env env' ->
-      forall n,
-        lookup env n = None -> lookup env' n = None.
-      intros A B env env' P P_env_env'; induction P_env_env';
-        destruct n; simpl; intros; try discriminate; auto.
-    Qed.
+  Lemma P2_Env_Nlookup A B (env : Env A) (env' : Env B) P :
+    P2_Env P env env' ->
+    forall n,
+      lookup env n = None -> lookup env' n = None.
+  Proof.
+    intros P_env_env'; induction P_env_env';
+      destruct n; simpl; intros; try discriminate; auto.
+  Qed.
 
-    Lemma P2_Env_Nlookup' : forall A B (env : Env A) (env' : Env B) P,
-      P2_Env P env env' ->
-      forall n,
-        lookup env' n = None -> lookup env n = None.
-      intros A B env env' P P_env_env'; induction P_env_env';
-        destruct n; simpl; intros; try discriminate; auto.
-    Qed.
+  Lemma P2_Env_Nlookup' A B (env : Env A) (env' : Env B) P :
+    P2_Env P env env' ->
+    forall n,
+      lookup env' n = None -> lookup env n = None.
+  Proof.
+    intros P_env_env'; induction P_env_env';
+      destruct n; simpl; intros; try discriminate; auto.
+  Qed.
 
-    Lemma P2_Env_length : forall A B (env : Env A) (env' : Env B) P,
-      P2_Env P env env' -> List.length env = List.length env'.
-      intros; induction H; simpl; congruence.
-    Qed.
+  Lemma P2_Env_length A B (env : Env A) (env' : Env B) P :
+    P2_Env P env env' -> List.length env = List.length env'.
+  Proof.
+    intros; induction H; simpl; congruence.
+  Qed.
 
-    Lemma P2_Env_insert : forall A B (env : Env A) (env' : Env B) (P : A -> B -> Prop),
-      P2_Env P env env' ->
-      forall a b, P a b -> P2_Env P (insert _ a env) (insert _ b env').
-      intros; induction H; simpl; constructor; eauto.
-      constructor.
-    Qed.
+  Lemma P2_Env_insert A B (env : Env A) (env' : Env B) (P : A -> B -> Prop) :
+    P2_Env P env env' ->
+    forall a b, P a b -> P2_Env P (insert _ a env) (insert _ b env').
+  Proof.
+    intros; induction H; simpl; constructor; eauto.
+    constructor.
+  Qed.
 
-    (* Need this better induction principle when we're reasoning about
+  (* Need this better induction principle when we're reasoning about
        Functors that use P2_Envs. *)
-    Definition P2_Env_ind' :=
+  Definition P2_Env_ind' :=
     fun (A B : Set) (P : A -> B -> Prop) (P0 : forall As Bs, P2_Env P As Bs -> Prop)
-      (f : P0 _ _ (P2_Nil _))
-      (f0 : forall (a : A) (b : B) (As : Env A) (Bs : Env B) (ABs : P2_Env P As Bs)
-        (P_a_b : P a b), P0 _ _ ABs -> P0 _ _ (P2_Cons P a b As Bs P_a_b ABs)) =>
-        fix F (env : Env A) (env0 : Env B) (p : P2_Env P env env0) {struct p} :
+        (f : P0 _ _ (P2_Nil _))
+        (f0 : forall (a : A) (b : B) (As : Env A) (Bs : Env B) (ABs : P2_Env P As Bs)
+                (P_a_b : P a b), P0 _ _ ABs -> P0 _ _ (P2_Cons P a b As Bs P_a_b ABs)) =>
+    fix F (env : Env A) (env0 : Env B) (p : P2_Env P env env0) {struct p} :
         P0 env env0 p :=
-        match p in (P2_Env _ env1 env2) return (P0 env1 env2 p) with
-        | P2_Nil => f
-        | P2_Cons a b As Bs y p0 => f0 a b As Bs p0 y (F As Bs p0)
-      end.
+    match p in (P2_Env _ env1 env2) return (P0 env1 env2 p) with
+      | P2_Nil => f
+      | P2_Cons a b As Bs y p0 => f0 a b As Bs p0 y (F As Bs p0)
+    end.
 
   (* ============================================== *)
   (* SUBVALUE RELATION                              *)
   (* ============================================== *)
 
+  Record SubValue_i : Set :=
+    mk_SubValue_i {sv_a : Value; sv_b : Value}.
 
-    Record SubValue_i : Set := mk_SubValue_i
-      {sv_a : Value;
-        sv_b : Value}.
+  (** SuperFunctor for SubValue Relation. **)
 
-    (** SuperFunctor for SubValue Relation. **)
+  Variable SV : (SubValue_i -> Prop) -> SubValue_i -> Prop.
+  Context `{ispf_SV : iSPF _ SV}.
+  Definition SubValue := iFix SV.
+  Definition SubValueC V1 V2:= SubValue (mk_SubValue_i V1 V2).
 
-    Variable SV : (SubValue_i -> Prop) -> SubValue_i -> Prop.
-    Context `{ispf_SV : iSPF _ SV}.
-    Definition SubValue := iFix SV.
-    Definition SubValueC V1 V2:= SubValue (mk_SubValue_i V1 V2).
+  (** Subvalue is reflexive **)
+  Inductive SubValue_refl (A : SubValue_i -> Prop) : SubValue_i -> Prop :=
+    SV_refl : forall v v',
+      v = v' ->
+      SubValue_refl A (mk_SubValue_i v v').
 
-    (** Subvalue is reflexive **)
-    Inductive SubValue_refl (A : SubValue_i -> Prop) : SubValue_i -> Prop :=
-      SV_refl : forall v v',
-        v = v' ->
-        SubValue_refl A (mk_SubValue_i v v').
+  Inductive SV_refl_S : SubValue_i -> Set :=
+    SSV_refl : forall v (v' : Value), v = v' -> SV_refl_S (mk_SubValue_i v v').
+  Inductive SV_refl_P : forall (i : SubValue_i), SV_refl_S i -> Set :=.
+  Definition SV_refl_R (i : SubValue_i) (s : SV_refl_S i) (p : SV_refl_P i s) :
+    SubValue_i := match p with end.
 
-    Inductive SV_refl_S : SubValue_i -> Set :=
-      SSV_refl : forall v (v' : Value), v = v' -> SV_refl_S (mk_SubValue_i v v').
-    Inductive SV_refl_P : forall (i : SubValue_i), SV_refl_S i -> Set :=.
-    Definition SV_refl_R (i : SubValue_i) (s : SV_refl_S i) (p : SV_refl_P i s) :
-      SubValue_i := match p with end.
-
-    Definition SV_refl_to A i : IExt _ _ SV_refl_R A i -> SubValue_refl A i :=
-      fun x =>
-        match x with
-          | iext s pf =>
-            match s with
-              | SSV_refl v v' e => SV_refl A v v' e
-            end
-        end.
-
-    Definition SV_refl_from A i : SubValue_refl A i -> IExt _ _ SV_refl_R A i :=
-      fun x => match
-        x in (SubValue_refl _ i) return (IExt SV_refl_S SV_refl_P SV_refl_R A i)
-      with
-        | SV_refl v v' e =>
-          iext _ _
-               (SSV_refl v v' e)
-               (fun p : SV_refl_P _ _ =>
-                  match p with end)
+  Definition SV_refl_to A i : IExt _ _ SV_refl_R A i -> SubValue_refl A i :=
+    fun x =>
+      match x with
+        | iext s pf =>
+          match s with
+            | SSV_refl v v' e => SV_refl A v v' e
+          end
       end.
 
+  Definition SV_refl_from A i : SubValue_refl A i -> IExt _ _ SV_refl_R A i :=
+    fun x => match
+      x in (SubValue_refl _ i) return (IExt SV_refl_S SV_refl_P SV_refl_R A i)
+    with
+      | SV_refl v v' e =>
+        iext _ _
+             (SSV_refl v v' e)
+             (fun p : SV_refl_P _ _ =>
+                match p with end)
+    end.
 
-    Global Instance SV_refl_Container : IContainer SubValue_refl :=
-      {| IS    := SV_refl_S;
-         IP    := SV_refl_P;
-         IR    := SV_refl_R;
-         ifrom := SV_refl_from;
-         ito   := SV_refl_to
-      |}.
-    Proof.
-      intros; destruct a; reflexivity.
-      intros; destruct a; destruct s; simpl.
-      f_equal; extensionality p; destruct p.
-    Defined.
+  Global Instance SV_refl_Container : IContainer SubValue_refl :=
+    {| IS    := SV_refl_S;
+       IP    := SV_refl_P;
+       IR    := SV_refl_R;
+       ifrom := SV_refl_from;
+       ito   := SV_refl_to
+    |}.
+  Proof.
+    intros; destruct a; reflexivity.
+    intros; destruct a; destruct s; simpl.
+    f_equal; extensionality p; destruct p.
+  Defined.
 
-    Definition ind_alg_SV_refl (P : SubValue_i -> Prop)
-      (H : forall v v', v = v' -> P (mk_SubValue_i v v'))
-      i (e : SubValue_refl P i) : P i :=
-      match e in SubValue_refl _ i return P i with
-        | SV_refl v v' eq_v => H v v' eq_v
-      end.
+  Definition ind_alg_SV_refl (P : SubValue_i -> Prop)
+    (H : forall v v', v = v' -> P (mk_SubValue_i v v'))
+    i (e : SubValue_refl P i) : P i :=
+    match e in SubValue_refl _ i return P i with
+      | SV_refl v v' eq_v => H v v' eq_v
+    end.
 
   Variable Sub_SV_refl_SV : Sub_iFunctor SubValue_refl SV.
 
@@ -533,6 +538,7 @@ Section Names.
 
   Variable Sub_SV_Bot_SV : Sub_iFunctor SubValue_Bot SV.
 
+
   (* Inversion principle for Bottom SubValues. *)
   Definition SV_invertBot_P (i : SubValue_i) :=
     sv_b i = bot -> sv_a i = bot.
@@ -543,6 +549,7 @@ Section Names.
 
   Global Instance SV_invertBot_refl :
     iPAlgebra SV_invertBot_Name SV_invertBot_P (SubValue_refl).
+  Proof.
     econstructor; intros.
     unfold iAlgebra; intros; unfold SV_invertBot_P.
     inversion H; subst; simpl; congruence.
@@ -550,6 +557,7 @@ Section Names.
 
   Global Instance SV_invertBot_Bot :
     iPAlgebra SV_invertBot_Name SV_invertBot_P SubValue_Bot.
+  Proof.
     econstructor; intros.
     unfold iAlgebra; intros; unfold SV_invertBot_P.
     inversion H; subst; simpl; eauto.
@@ -562,8 +570,8 @@ Section Names.
   Definition Sub_Environment (env env' : Env _) :=
     P2_Env SubValueC env env'.
 
-  Lemma Sub_Environment_refl : forall (env : Env _),
-    Sub_Environment env env.
+  Lemma Sub_Environment_refl (env : Env _) : Sub_Environment env env.
+  Proof.
     induction env; econstructor; eauto.
     apply (inject_i (subGF := Sub_SV_refl_SV));
       constructor; reflexivity.
@@ -573,221 +581,224 @@ Section Names.
   (* EVALUATION IS CONTINUOUS                        *)
   (* ============================================== *)
 
-    (** Helper property for proof of continuity of evaluation. **)
-    Definition eval_continuous_Exp_P (e : Exp) :=
-      forall (m : nat),
-        (forall (e0 : Exp)
-          (gamma gamma' : Env Value) (n : nat),
-          Sub_Environment gamma gamma' ->
-          m <= n -> SubValueC (beval m e0 gamma) (beval n e0 gamma')) ->
-        forall (gamma gamma' : Env Value) (n : nat),
-          Sub_Environment gamma gamma' ->
-          m <= n ->
-          SubValueC (beval (S m) e gamma) (beval (S n) e gamma').
+  (** Helper property for proof of continuity of evaluation. **)
+  Definition eval_continuous_Exp_P (e : Exp) :=
+    forall (m : nat),
+      (forall (e0 : Exp) (gamma gamma' : Env Value) (n : nat),
+         Sub_Environment gamma gamma' ->
+         m <= n -> SubValueC (beval m e0 gamma) (beval n e0 gamma')) ->
+      forall (gamma gamma' : Env Value) (n : nat),
+        Sub_Environment gamma gamma' ->
+        m <= n ->
+        SubValueC (beval (S m) e gamma) (beval (S n) e gamma').
 
-    Inductive EC_ExpName := ec_expname.
+  Inductive EC_ExpName := ec_expname.
 
-    Context {eval_continuous_Exp_E :
-      FPAlgebra (eval_continuous_Exp_P) (inject E E)}.
+  Context {eval_continuous_Exp_E :
+    FPAlgebra (eval_continuous_Exp_P) (inject E E)}.
 
-    (** Evaluation is continuous. **)
-    Lemma beval_continuous : forall m,
-      forall (e : Exp) (gamma gamma' : Env _),
-        forall n (Sub_G_G' : Sub_Environment gamma gamma'),
-          m <= n ->
-          SubValueC (beval m e gamma) (beval n e gamma').
-      induction m; simpl.
-      intros; eapply in_ti; eapply inj_i; econstructor; simpl; eauto.
-      intros; destruct n; try (inversion H; fail).
-      assert (m <= n) as le_m_n0 by auto with arith; clear H.
-      revert m IHm gamma gamma' n Sub_G_G' le_m_n0.
-      fold (eval_continuous_Exp_P e).
-      apply Ind.
-    Qed.
+  (** Evaluation is continuous. **)
+  Lemma beval_continuous :
+    forall m (e : Exp) (gamma gamma' : Env _),
+    forall n (Sub_G_G' : Sub_Environment gamma gamma'),
+      m <= n ->
+      SubValueC (beval m e gamma) (beval n e gamma').
+  Proof.
+    induction m; simpl.
+    intros; eapply in_ti; eapply inj_i; econstructor; simpl; eauto.
+    intros; destruct n; try (inversion H; fail).
+    assert (m <= n) as le_m_n0 by auto with arith; clear H.
+    revert m IHm gamma gamma' n Sub_G_G' le_m_n0.
+    fold (eval_continuous_Exp_P e).
+    apply Ind.
+  Qed.
 
   (* ============================================== *)
   (* WELL-FORMED VALUES RELATION                     *)
   (* ============================================== *)
 
-    Record WFValue_i : Set := mk_WFValue_i
-      {wfv_a : Value;
-        wfv_b : DType}.
+  Record WFValue_i : Set :=
+    mk_WFValue_i {wfv_a : Value; wfv_b : DType}.
 
-    (** SuperFunctor for Well-Formed Value Relation. **)
+  (** SuperFunctor for Well-Formed Value Relation. **)
 
-    Variable WFV : (WFValue_i -> Prop) -> WFValue_i -> Prop.
-    Context `{ispf_WFV : iSPF _ WFV}.
-    Definition WFValue := iFix WFV.
-    Definition WFValueC V T:= WFValue (mk_WFValue_i V T).
+  Variable WFV : (WFValue_i -> Prop) -> WFValue_i -> Prop.
+  Context `{ispf_WFV : iSPF _ WFV}.
+  Definition WFValue := iFix WFV.
+  Definition WFValueC V T:= WFValue (mk_WFValue_i V T).
 
-    (** Bottom is well-formed **)
+  (** Bottom is well-formed **)
 
-    Inductive WFValue_Bot (A : WFValue_i -> Prop) : WFValue_i -> Prop :=
-      WFV_Bot : forall v T,
-        v = inject BotValue V (Bot _) ->
-        WFValue_Bot A (mk_WFValue_i v T).
+  Inductive WFValue_Bot (A : WFValue_i -> Prop) : WFValue_i -> Prop :=
+    WFV_Bot : forall v T,
+      v = inject BotValue V (Bot _) ->
+      WFValue_Bot A (mk_WFValue_i v T).
 
-    Inductive WFV_Bot_S : WFValue_i -> Set :=
-      SWFV_Bot : forall v T,
-      v = bot ->
-      WFV_Bot_S (mk_WFValue_i v T).
+  Inductive WFV_Bot_S : WFValue_i -> Set :=
+    SWFV_Bot : forall v T,
+    v = bot ->
+    WFV_Bot_S (mk_WFValue_i v T).
 
-    Inductive WFV_Bot_P : forall (i : WFValue_i), WFV_Bot_S i -> Set :=.
-    Definition WFV_Bot_R (i : WFValue_i) (s : WFV_Bot_S i) (p : WFV_Bot_P i s) :
-      WFValue_i := match p with end.
+  Inductive WFV_Bot_P : forall (i : WFValue_i), WFV_Bot_S i -> Set :=.
+  Definition WFV_Bot_R (i : WFValue_i) (s : WFV_Bot_S i) (p : WFV_Bot_P i s) :
+    WFValue_i := match p with end.
 
-    Definition WFV_Bot_to A i : IExt _ _ WFV_Bot_R A i -> WFValue_Bot A i :=
-      fun x =>
-        match x with
-          | iext s pf =>
-            match s with
-              | SWFV_Bot v T eq => WFV_Bot A v T eq
-            end
-        end.
-
-    Definition WFV_Bot_from A i : WFValue_Bot A i -> IExt _ _ WFV_Bot_R A i :=
-      fun x => match
-        x in (WFValue_Bot _ i) return (IExt _ _ WFV_Bot_R A i)
-      with
-        | WFV_Bot v T eq =>
-          iext _ _
-               (SWFV_Bot v T eq)
-               (fun p : WFV_Bot_P _ _ =>
-                  match p with end)
+  Definition WFV_Bot_to A i : IExt _ _ WFV_Bot_R A i -> WFValue_Bot A i :=
+    fun x =>
+      match x with
+        | iext s pf =>
+          match s with
+            | SWFV_Bot v T eq => WFV_Bot A v T eq
+          end
       end.
 
-    Global Instance WFV_Bot_Container : IContainer WFValue_Bot :=
-      {| IS    := WFV_Bot_S;
-         IP    := WFV_Bot_P;
-         IR    := WFV_Bot_R;
-         ifrom := WFV_Bot_from;
-         ito   := WFV_Bot_to
-      |}.
-    Proof.
-      intros; destruct a; reflexivity.
-      intros; destruct a; destruct s; simpl.
-      f_equal; extensionality p; destruct p.
-    Defined.
+  Definition WFV_Bot_from A i : WFValue_Bot A i -> IExt _ _ WFV_Bot_R A i :=
+    fun x => match
+      x in (WFValue_Bot _ i) return (IExt _ _ WFV_Bot_R A i)
+    with
+      | WFV_Bot v T eq =>
+        iext _ _
+             (SWFV_Bot v T eq)
+             (fun p : WFV_Bot_P _ _ =>
+                match p with end)
+    end.
 
-    Variable WF_WFV_Bot_WFV : Sub_iFunctor WFValue_Bot WFV.
+  Global Instance WFV_Bot_Container : IContainer WFValue_Bot :=
+    {| IS    := WFV_Bot_S;
+       IP    := WFV_Bot_P;
+       IR    := WFV_Bot_R;
+       ifrom := WFV_Bot_from;
+       ito   := WFV_Bot_to
+    |}.
+  Proof.
+    intros; destruct a; reflexivity.
+    intros; destruct a; destruct s; simpl.
+    f_equal; extensionality p; destruct p.
+  Defined.
 
-    Definition WF_Environment env env' :=
-      P2_Env (fun v T =>
-        match T with
-          | Some T => WFValueC v T
-          | None => False
-        end) env env'.
+  Variable WF_WFV_Bot_WFV : Sub_iFunctor WFValue_Bot WFV.
+
+  Definition WF_Environment env env' :=
+    P2_Env (fun v T =>
+      match T with
+        | Some T => WFValueC v T
+        | None => False
+      end) env env'.
 
   (* ============================================== *)
   (* Evaluation preserves Well-Formedness           *)
   (* ============================================== *)
 
-    Definition WF_Value_continuous_P i :=
-      forall T, WFValueC (sv_b i) T -> WFValueC (sv_a i) T.
+  Definition WF_Value_continuous_P i :=
+    forall T, WFValueC (sv_b i) T -> WFValueC (sv_a i) T.
 
-    Inductive WFV_ContinuousName : Set := wfv_continuousname.
+  Inductive WFV_ContinuousName : Set := wfv_continuousname.
 
-    Context {WF_Value_continous_alg : iPAlgebra WFV_ContinuousName WF_Value_continuous_P SV}.
+  Context {WF_Value_continous_alg : iPAlgebra WFV_ContinuousName WF_Value_continuous_P SV}.
 
-    Global Instance WFV_Value_continuous_refl  :
-      iPAlgebra WFV_ContinuousName WF_Value_continuous_P SubValue_refl.
-      constructor; unfold iAlgebra; intros.
-      inversion H; subst.
-      unfold WF_Value_continuous_P. auto.
-    Qed.
+  Global Instance WFV_Value_continuous_refl  :
+    iPAlgebra WFV_ContinuousName WF_Value_continuous_P SubValue_refl.
+  Proof.
+    constructor; unfold iAlgebra; intros.
+    inversion H; subst.
+    unfold WF_Value_continuous_P. auto.
+  Qed.
 
-    Global Instance WFV_Value_continuous_Bot  :
-      iPAlgebra WFV_ContinuousName WF_Value_continuous_P SubValue_Bot.
-      constructor; unfold iAlgebra; intros.
-      inversion H; subst.
-      unfold WF_Value_continuous_P; simpl; intros.
-      apply inject_i; constructor; auto.
-    Qed.
+  Global Instance WFV_Value_continuous_Bot  :
+    iPAlgebra WFV_ContinuousName WF_Value_continuous_P SubValue_Bot.
+  Proof.
+    constructor; unfold iAlgebra; intros.
+    inversion H; subst.
+    unfold WF_Value_continuous_P; simpl; intros.
+    apply inject_i; constructor; auto.
+  Qed.
 
-    Lemma WF_Value_continous : forall v v',
-      SubValueC v v' ->
-      WF_Value_continuous_P (mk_SubValue_i v v').
-      intros; apply (ifold_ ); try assumption.
-      apply if_algebra.
-    Qed.
+  Lemma WF_Value_continous v v' :
+    SubValueC v v' ->
+    WF_Value_continuous_P (mk_SubValue_i v v').
+  Proof.
+    intros; apply ifold_; try assumption.
+    apply if_algebra.
+  Qed.
 
-    Lemma WF_Value_beval : forall m n,
-      forall (e : Exp) gamma gamma' T
-        (Sub_G_G' : Sub_Environment gamma' gamma),
-        m <= n ->
-        WFValueC (beval n e gamma) T ->
-        WFValueC (beval m e gamma') T.
-      intros; eapply WF_Value_continous.
-      eapply beval_continuous; try eassumption.
-      eassumption.
-    Qed.
+  Lemma WF_Value_beval m n (e : Exp) gamma gamma' T :
+      Sub_Environment gamma' gamma ->
+      m <= n ->
+      WFValueC (beval n e gamma) T ->
+      WFValueC (beval m e gamma') T.
+  Proof.
+    intros; eapply WF_Value_continous.
+    eapply beval_continuous; try eassumption.
+    eassumption.
+  Qed.
 
-    Variable (WF_MAlg_typeof : WF_MAlgebra Typeof_E).
-    Variable (WF_MAlg_eval : WF_MAlgebra eval_E).
+  Variable (WF_MAlg_typeof : WF_MAlgebra Typeof_E).
+  Variable (WF_MAlg_eval : WF_MAlgebra eval_E).
 
-    Definition eval_alg_Soundness_P
-      (P_bind : Set)
-      (P : P_bind -> Env Value -> Prop)
-      (E' : Set -> Set)
-      `{spf_E' : SPF E'}
-      (pb : P_bind)
-      (typeof_rec : Fix E' -> typeofR)
-      (eval_rec : Exp -> evalR)
-      (typeof_F : Mixin (Fix E') E' typeofR)
-      (eval_F : Mixin Exp E evalR)
-      (e : (Fix E') * (Fix E)) :=
-      forall
-      gamma'' (WF_gamma'' : P pb gamma'')
-      (IHa : forall pb gamma'' (WF_gamma'' : P pb gamma'') (a : (Fix E' * Exp)),
-          (forall T,
-            typeof_F typeof_rec (out_t (fst a)) = Some T ->
-            WFValueC (eval_F eval_rec (out_t (snd a)) gamma'') T) ->
-          forall T, typeof_rec (fst a) = Some T ->
-            WFValueC (eval_rec (snd a) gamma'') T),
-        forall T : DType,
-          typeof_F typeof_rec (out_t (fst e)) = Some T ->
-          WFValueC (eval_F eval_rec (out_t (snd e)) gamma'') T.
+  Definition eval_alg_Soundness_P
+    (P_bind : Set)
+    (P : P_bind -> Env Value -> Prop)
+    (E' : Set -> Set)
+    `{spf_E' : SPF E'}
+    (pb : P_bind)
+    (typeof_rec : Fix E' -> typeofR)
+    (eval_rec : Exp -> evalR)
+    (typeof_F : Mixin (Fix E') E' typeofR)
+    (eval_F : Mixin Exp E evalR)
+    (e : (Fix E') * (Fix E)) :=
+    forall
+    gamma'' (WF_gamma'' : P pb gamma'')
+    (IHa : forall pb gamma'' (WF_gamma'' : P pb gamma'') (a : (Fix E' * Exp)),
+        (forall T,
+          typeof_F typeof_rec (out_t (fst a)) = Some T ->
+          WFValueC (eval_F eval_rec (out_t (snd a)) gamma'') T) ->
+        forall T, typeof_rec (fst a) = Some T ->
+          WFValueC (eval_rec (snd a) gamma'') T),
+      forall T : DType,
+        typeof_F typeof_rec (out_t (fst e)) = Some T ->
+        WFValueC (eval_F eval_rec (out_t (snd e)) gamma'') T.
 
-    Context {eval_Soundness_alg_F : forall typeof_rec eval_rec,
-      FPAlgebra (eval_alg_Soundness_P unit (fun _ _ => True) _ tt
-        typeof_rec eval_rec
-        (f_algebra TypeofName (FAlgebra := Typeof_E _))
-        (f_algebra EvalName (FAlgebra := eval_E _))) (inject2 E E E)}.
+  Context {eval_Soundness_alg_F : forall typeof_rec eval_rec,
+    FPAlgebra (eval_alg_Soundness_P unit (fun _ _ => True) E tt
+      typeof_rec eval_rec
+      (f_algebra TypeofName (FAlgebra := Typeof_E _))
+      (f_algebra EvalName (FAlgebra := eval_E _))) (inject2 E E E)}.
 
-    Lemma eval_Soundness : forall (e : Exp),
-      forall gamma'' T, typeof e = Some T ->
-        WFValueC (eval e gamma'') T.
-      intros.
-      rewrite <- (@in_out_inverse _ _ _ _ e).
-      unfold eval; rewrite fold_computation; fold eval.
-      rewrite wf_malgebra.
-      unfold id.
-      try rewrite <- eta_expansion.
-      apply (Ind2 (Ind_Alg := eval_Soundness_alg_F typeof eval)); auto.
-      destruct a; simpl.
-      intros.
-      rewrite <- (@in_out_inverse _ _ _ _ e0).
-      unfold eval; rewrite fold_computation; fold eval.
-      rewrite wf_malgebra.
-      unfold id.
-      try rewrite <- eta_expansion.
-      apply H0.
-      unfold typeof in H1.
-      rewrite <- (@in_out_inverse _ _ _ _ f) in H1.
-      rewrite fold_computation in H1.
-      rewrite wf_malgebra in H1.
-      unfold id in H1.
-      try rewrite <- eta_expansion in H1.
-      apply H1.
-      simpl.
-      unfold typeof in H.
-      rewrite <- (@in_out_inverse _ _ _ _ e) in H.
-      rewrite fold_computation in H.
-      rewrite wf_malgebra in H.
-      unfold id in H.
-      try rewrite <- eta_expansion in H.
-      apply H.
-    Qed.
+  Lemma eval_Soundness (e : Exp) gamma'' T :
+    typeof e = Some T ->
+    WFValueC (eval e gamma'') T.
+  Proof.
+    intros.
+    rewrite <- (@in_out_inverse _ _ _ _ e).
+    unfold eval; rewrite fold_computation; fold eval.
+    rewrite wf_malgebra.
+    unfold id.
+    try rewrite <- eta_expansion.
+    apply (Ind2 (Ind_Alg := eval_Soundness_alg_F typeof eval)); auto.
+    destruct a; simpl.
+    intros.
+    rewrite <- (@in_out_inverse _ _ _ _ e0).
+    unfold eval; rewrite fold_computation; fold eval.
+    rewrite wf_malgebra.
+    unfold id.
+    try rewrite <- eta_expansion.
+    apply H0.
+    unfold typeof in H1.
+    rewrite <- (@in_out_inverse _ _ _ _ f) in H1.
+    rewrite fold_computation in H1.
+    rewrite wf_malgebra in H1.
+    unfold id in H1.
+    try rewrite <- eta_expansion in H1.
+    apply H1.
+    simpl.
+    unfold typeof in H.
+    rewrite <- (@in_out_inverse _ _ _ _ e) in H.
+    rewrite fold_computation in H.
+    rewrite wf_malgebra in H.
+    unfold id in H.
+    try rewrite <- eta_expansion in H.
+    apply H.
+  Qed.
 
 End Names.
 
