CaseStudy/test_AL.v
@@ -1,13 +1,10 @@
-Require Import String.
-Require Import GDTC.Polynomial.
-Require Import GDTC.Containers.
-Require Import GDTC.Functors.
+Require Import Coq.Strings.String.
+Require Import GDTC.
 Require Import CaseStudy.Names.
 Require Import CaseStudy.PNames.
 Require Import CaseStudy.Arith.
 Require Import CaseStudy.Lambda.
 Require Import CaseStudy.Arith_Lambda.
-(* Require Import MonadLib. *)
 
 Open Scope string_scope.
 
@@ -22,7 +19,7 @@ End Type_Test_Section.
 
 Section Test_Section.
 
-  Definition E (A : Set) := Arith :+: (Lambda D A).
+  Definition E (A: Set) := Arith :+: (Lambda D A).
 
   Global Instance Container_E : forall (A : Set), Container (E A).
     eauto with typeclass_instances.
@@ -38,11 +35,8 @@ Section Test_Section.
     eauto with typeclass_instances.
   Defined.
 
-  Instance V_eval : FAlgebra EvalName (Names.Exp (E nat)) (evalR V) (E nat).
-    apply FAlgebra_Plus.
+  Instance V_eval : FAlgebra EvalName (Exp E nat) (evalR V) (E nat).
     eauto 150 with typeclass_instances.
-    generalize (MAlgebra_eval_Lambda D E V).
-    simpl; auto.
   Defined.
 
   Definition SV := (SubValue_refl V) ::+:: (SubValue_Bot V) ::+:: (SubValue_Clos E V).
@@ -51,43 +45,16 @@ Section Test_Section.
     eauto with typeclass_instances.
   Defined.
 
-  Global Instance SV_invertVI_SV :
-    iPAlgebra SV_invertVI_Name (SV_invertVI_P V) SV.
-    repeat apply iPAlgebra_Plus; eauto 150 with typeclass_instances.
-    constructor.
-    unfold iAlgebra.
-    unfold SV_invertVI_P.
-    intros i H n H0.
-    inversion H; subst.
-    elimtype False; apply (inject_discriminate _ _ _ H0).
-  Defined.
-
-  Global Instance SV_invertVI'_SV :
-    iPAlgebra SV_invertVI'_Name (SV_invertVI'_P V) SV.
-    repeat apply iPAlgebra_Plus; eauto 150 with typeclass_instances.
-    constructor.
-    unfold iAlgebra.
-    unfold SV_invertVI'_P.
-    intros i H n H0.
-    inversion H; subst.
-    elimtype False; apply (inject_discriminate _ _ _ H0).
-  Defined.
-
-  Global Instance SV_invertBot_SV :
-    iPAlgebra SV_invertBot_Name (SV_invertBot_P V) SV.
-    repeat apply iPAlgebra_Plus; eauto 150 with typeclass_instances.
-  Defined.
-
   Global Instance EV_Alg :
     FPAlgebra (eval_continuous_Exp_P V (E nat) SV) (inject (E nat) (E nat)).
   Proof.
     apply FPAlgebra_Plus_cont_inject; eauto 200 with typeclass_instances.
-    - generalize (@Lambda_eval_continuous_Exp D _ _ _ E _ _ _ _).
+    - pose proof (Lambda_eval_continuous_Exp D E).
       eauto 200 with typeclass_instances.
   Qed.
 
-  Definition eval_continuous : forall m,
-    forall (e : Names.Exp (E nat)) (gamma gamma' : Env _),
+  Lemma eval_continuous : forall m,
+    forall (e : Exp E nat) (gamma gamma' : Env _),
       forall n (Sub_G_G' : Sub_Environment V SV gamma gamma'),
         m <= n ->
         SubValueC _ SV (beval _ _ m e gamma) (beval _ _ n e gamma').
@@ -97,7 +64,6 @@ Section Test_Section.
   Eval compute in ("Continuity of Evaluation Proven!").
 
   Definition Eqv (A B : Set) := (NP_Functor_eqv E Arith A B) ::+:: (Lambda_eqv D E A B).
-
   Global Instance Container_Eqv : forall (A B : Set), IContainer (Eqv A B).
     eauto with typeclass_instances.
   Defined.
@@ -106,30 +72,20 @@ Section Test_Section.
     (WFValue_Bot D V) ::+:: (WFValue_VI D V).
 
   Global Instance Container_WFV : IContainer WFV.
-    repeat apply IContainerSum; eauto with typeclass_instances.
+    eauto with typeclass_instances.
   Defined.
 
-  Instance Eval_Soundness_alg :
-    forall
-      eval_rec : Names.Exp (E nat) -> evalR V,
-      iPAlgebra soundness_XName
-                (soundness_X'_P D V E Eqv WFV
-                                (typeof D (E (typeofR D))) eval_rec
-                                (f_algebra TypeofName) (f_algebra EvalName))
-                (Eqv (typeofR D) nat).
-  Proof.
-    assert (WF_FAlgebra_eval_Lambda :
-              WF_FAlgebra EvalName (Names.Exp (E nat)) (evalR V)
-                (Lambda D nat) (E nat) (MAlgebra_eval_Lambda D E V) V_eval).
-    eauto with typeclass_instances.
-    intros.
-    repeat apply iPAlgebra_Plus.
-    apply Lift_soundness_X_alg.
-    eauto with typeclass_instances.
-    apply eqv_eval_Soundness;
-    eauto 250 with typeclass_instances.
-    apply (@Lambda_eqv_eval_soundness_alg D _ _ _ _ _ E _ _ _ _ V _ _ _ _ _ _ _ V_eval WF_FAlgebra_eval_Lambda _ _ Eqv _ _ _ _ WFV _ _ (typeof D (E (typeofR D)))); eauto with typeclass_instances.
-    eauto 250 with typeclass_instances.
+  Instance Eval_Soundness_alg (eval_rec : Exp E nat -> evalR V) :
+    iPAlgebra soundness_XName
+              (soundness_X'_P D V E Eqv WFV
+                              (typeof D (E (typeofR D))) eval_rec
+                              (f_algebra TypeofName) (f_algebra EvalName))
+              (Eqv (typeofR D) nat).
+  Proof with eauto 200 with typeclass_instances.
+    repeat apply iPAlgebra_Plus...
+    - apply Lift_soundness_X_alg...
+      apply eqv_eval_Soundness...
+    - pose proof (Lambda_eqv_eval_soundness_alg D E)...
   Qed.
 
   Theorem soundness : forall n gamma gamma' gamma'' e' e'',
@@ -141,7 +97,7 @@ Section Test_Section.
     (WF_gamma'' : WF_Environment _ _ WFV gamma'' gamma) T,
     typeof D (E _) e' = Some T -> WFValueC _ _ WFV (beval _ _ n e'' gamma'') T.
   Proof.
-    apply (soundness_X D V E Eqv WFV _ _ SV).
+    eapply soundness_X; eauto 350 with typeclass_instances.
   Qed.
 
   Eval compute in ("Type Soundness for Arith :+: Lambda Proven!").
