CaseStudy/test_BL.v
@@ -1,13 +1,10 @@
-Require Import String.
-Require Import GDTC.Polynomial.
-Require Import GDTC.Containers.
-Require Import GDTC.Functors.
+Require Import Coq.Strings.String.
+Require Import GDTC.
 Require Import CaseStudy.Names.
 Require Import CaseStudy.PNames.
 Require Import CaseStudy.Bool.
 Require Import CaseStudy.Lambda.
 Require Import CaseStudy.Bool_Lambda.
-(* Require Import MonadLib. *)
 
 Open Scope string_scope.
 
@@ -22,7 +19,7 @@ End Type_Test_Section.
 
 Section Test_Section.
 
-  Definition E (A : Set) := Bool :+: (Lambda D A).
+  Definition E (A: Set) := Bool :+: (Lambda D A).
 
   Global Instance Container_E : forall (A : Set), Container (E A).
     eauto with typeclass_instances.
@@ -34,6 +31,10 @@ Section Test_Section.
 
   Definition V := StuckValue :+: BotValue :+: (ClosValue E) :+: BoolValue.
 
+  Global Instance Container_V : Container V.
+    eauto with typeclass_instances.
+  Defined.
+
   Instance V_eval : FAlgebra EvalName (Exp E nat) (evalR V) (E nat).
     eauto 150 with typeclass_instances.
   Defined.
@@ -44,47 +45,20 @@ Section Test_Section.
     eauto with typeclass_instances.
   Defined.
 
-  Global Instance SV_invertVB_SV :
-    iPAlgebra SV_invertVB_Name (SV_invertVB_P V) SV.
-    repeat apply iPAlgebra_Plus; eauto 150 with typeclass_instances.
-    constructor.
-    unfold iAlgebra.
-    unfold SV_invertVB_P.
-    intros i H n H0.
-    inversion H; subst.
-    elimtype False; apply (inject_discriminate _ _ _ H0).
-  Defined.
-
-  Global Instance SV_invertVB'_SV :
-    iPAlgebra SV_invertVB'_Name (SV_invertVB'_P V) SV.
-    repeat apply iPAlgebra_Plus; eauto 150 with typeclass_instances.
-    constructor.
-    unfold iAlgebra.
-    unfold SV_invertVB'_P.
-    intros i H n H0.
-    inversion H; subst.
-    elimtype False; apply (inject_discriminate _ _ _ H0).
-  Defined.
-
-  Global Instance SV_invertBot_SV :
-    iPAlgebra SV_invertBot_Name (SV_invertBot_P V) SV.
-    repeat apply iPAlgebra_Plus; eauto 150 with typeclass_instances.
-  Defined.
-
   Global Instance EV_Alg :
     FPAlgebra (eval_continuous_Exp_P V (E nat) SV) (inject (E nat) (E nat)).
   Proof.
     apply FPAlgebra_Plus_cont_inject; eauto 200 with typeclass_instances.
-    - generalize (@Lambda_eval_continuous_Exp D _ _ _ E _ _ _ _).
+    - pose proof (Lambda_eval_continuous_Exp D E).
       eauto 200 with typeclass_instances.
   Qed.
 
-  Definition eval_continuous : forall m,
+  Lemma eval_continuous : forall m,
     forall (e : Exp E nat) (gamma gamma' : Env _),
       forall n (Sub_G_G' : Sub_Environment V SV gamma gamma'),
         m <= n ->
         SubValueC _ SV (beval _ _ m e gamma) (beval _ _ n e gamma').
-    eapply beval_continuous; eauto with typeclass_instances.
+    apply beval_continuous; eauto with typeclass_instances.
   Qed.
 
   Eval compute in ("Continuity of Evaluation Proven!").
@@ -101,39 +75,18 @@ Section Test_Section.
     eauto with typeclass_instances.
   Defined.
 
-  Instance Eval_Soundness_alg :
-    forall
-      eval_rec : Names.Exp (E nat) -> evalR V,
-      iPAlgebra soundness_XName
-                (soundness_X'_P D V E Eqv WFV
-                                (typeof D (E (typeofR D))) eval_rec
-                                (f_algebra TypeofName) (f_algebra EvalName))
-                (Eqv (typeofR D) nat).
-  Proof.
-    assert (WF_FAlgebra_eval_Lambda :
-              WF_FAlgebra EvalName (Names.Exp (E nat)) (evalR V)
-                (Lambda D nat) (E nat) (MAlgebra_eval_Lambda D E V) V_eval).
-    eauto with typeclass_instances.
-    intros.
-    repeat apply iPAlgebra_Plus.
-    apply Lift_soundness_X_alg.
-    eauto with typeclass_instances.
-    apply eqv_eval_Soundness;
-    eauto 250 with typeclass_instances.
-    apply (@Lambda_eqv_eval_soundness_alg D _ _ _ _ _ E _ _ _ _ V _ _ _ _ _ _ _ V_eval WF_FAlgebra_eval_Lambda _ _ Eqv _ _ _ _ WFV _ _ (typeof D (E (typeofR D)))); eauto with typeclass_instances.
-    eauto 250 with typeclass_instances.
+  Instance Eval_Soundness_alg (eval_rec : Exp E nat -> evalR V) :
+    iPAlgebra soundness_XName
+              (soundness_X'_P D V E Eqv WFV
+                              (typeof D (E (typeofR D))) eval_rec
+                              (f_algebra TypeofName) (f_algebra EvalName))
+              (Eqv (typeofR D) nat).
+  Proof with eauto 200 with typeclass_instances.
+    repeat apply iPAlgebra_Plus...
+    apply Lift_soundness_X_alg...
+    apply eqv_eval_Soundness...
+    pose proof (Lambda_eqv_eval_soundness_alg D E)...
   Qed.
-
-  (*
-  Global Instance Bool_Soundness_alg P_bind P pb typeof_rec eval_rec :
-    PAlgebra eval_Soundness_alg_Name
-    (sig (UP'_P2 (eval_alg_Soundness_P D V (E nat) WFV P_bind P
-      (E (typeofR D)) (Functor_Plus Bool (Lambda D (typeofR D))) pb typeof_rec eval_rec
-      f_algebra f_algebra))) Bool.
-  Proof.
-    eauto 100 with typeclass_instances.
-  Defined.
-  *)
 
   Theorem soundness : forall n gamma gamma' gamma'' e' e'',
     E_eqvC _ Eqv gamma gamma' e' e'' ->
