CaseStudy/Bool_Lambda.v
@@ -1,77 +1,62 @@
 Require Import Coq.Program.Equality.
-Require Import List.
-Require Import FunctionalExtensionality.
-Require Import GDTC.FJ_tactics.
-Require Import GDTC.Polynomial.
-Require Import GDTC.Containers.
-Require Import GDTC.Functors.
-Require Import CaseStudy.Names.
-Require Import CaseStudy.PNames.
+Require Import GDTC.
 Require Import CaseStudy.Bool.
 Require Import CaseStudy.Lambda.
+Require Import CaseStudy.Names.
+Require Import CaseStudy.PNames.
 
 Section PLambda_Bool.
 
   Variable D : Set -> Set.
-  Context {Fun_D : Functor D}.
-  Context {PFun_D : PFunctor D}.
-  Context {SPF_D : SPF D}.
+  Context `{spf_D : SPF D}.
   Context {Sub_BType_D : BType :<: D}.
   Context {Sub_LType_D : LType :<: D}.
   Context {WF_Sub_BType_D : WF_Functor _ _ Sub_BType_D}.
   Context {WF_Sub_LType_D : WF_Functor _ _ Sub_LType_D}.
 
   Variable E : Set -> Set -> Set.
-  Context {Fun_E : forall A, Functor (E A)}.
-  Context {PFun_E : forall A, PFunctor (E A)}.
-  Context {SPF_E : forall A, SPF (E A)}.
+  Context {fun_E : forall A, Functor (E A)}.
+  Context {pfun_E: forall A, PFunctor (E A)}.
+  Context {spf_E : forall A, SPF (E A)}.
   Context {Sub_Bool_E : forall A, Bool :<: (E A)}.
-  Context {Typeof_F : forall T, FAlgebra TypeofName T (typeofR D) (E (typeofR D))}.
+
   Variable EQV_E : forall A B, (eqv_i E A B -> Prop) -> eqv_i E A B -> Prop.
-  Context {funEQV_E : forall A B, iFunctor (EQV_E A B)}.
+  Context {ifun_EQV_E : forall A B, iFunctor (EQV_E A B)}.
   Context {ispf_EQV_E : forall A B, iSPF (EQV_E A B)}.
 
   Variable V : Set -> Set.
-  Context {Fun_V : Functor V}.
-  Context {PFun_V : PFunctor V}.
-  Context {SPF_V : SPF V}.
+  Context `{spf_V : SPF V}.
   Context {Sub_BoolValue_V : BoolValue :<: V}.
   Context {Sub_BotValue_V : BotValue :<: V}.
   Context {Sub_ClosValue_V : ClosValue E :<: V}.
-  Context {Sub_StuckValue_V : StuckValue :<: V}.
-  Variable WFV : (WFValue_i D V -> Prop) -> WFValue_i D V -> Prop.
-  Context {funWFV : iFunctor WFV}.
-  Context {ispf_WFV : iSPF WFV}.
 
-  Context {Sub_WFV_VB_WFV : Sub_iFunctor (WFValue_VB D V) WFV}.
-  Context {Sub_WFV_Bot_WFV : Sub_iFunctor (WFValue_Bot D V) WFV}.
-  Context {Dis_Clos_Bot : Distinct_Sub_Functor LType BType D}.
+  Variable WFV : (WFValue_i D V -> Prop) -> WFValue_i D V -> Prop.
+  Context `{spfWFV : iSPF _ WFV}.
 
   Context {Dis_VB_Clos : Distinct_Sub_Functor BoolValue (ClosValue E) V}.
   Context {WF_Sub_ClosValue_V : WF_Functor (ClosValue E) V Sub_ClosValue_V}.
   Context {WF_Sub_BoolValue_V : WF_Functor BoolValue V Sub_BoolValue_V}.
 
+  Context {Sub_WFV_VB_WFV : Sub_iFunctor (WFValue_VB D V) WFV}.
+  Context {Dis_LType_BType : Distinct_Sub_Functor LType BType D}.
+
   Global Instance PAlgebra_WF_invertClos_VB typeof_rec :
     iPAlgebra WF_invertClos_Name (WF_invertClos_P D E V EQV_E WFV typeof_rec) (WFValue_VB D V).
   Proof.
-    econstructor; intros.
-    unfold iAlgebra; intros; unfold WF_invertClos_P.
-    inversion H; subst; simpl; intros.
-    split.
-    apply (inject_i (subGF := Sub_WFV_VB_WFV)); econstructor; eauto.
-    intros; discriminate_inject H0.
-  Defined.
+    constructor; unfold iAlgebra, WF_invertClos_P.
+    inversion 1; subst; simpl; split.
+    - apply (inject_i (subGF := Sub_WFV_VB_WFV)); econstructor; eauto.
+    - intros ? ? Heq; discriminate_inject Heq.
+  Qed.
 
   Global Instance PAlgebra_WF_invertClos'_VB typeof_rec :
     iPAlgebra WF_invertClos'_Name (WF_invertClos'_P D E V EQV_E WFV typeof_rec) (WFValue_VB D V).
   Proof.
-    econstructor; intros.
-    unfold iAlgebra; intros; unfold WF_invertClos_P.
-    inversion H; subst; simpl; intros.
-    split.
-    apply (inject_i (subGF := Sub_WFV_VB_WFV)); econstructor; eauto.
-    intros; discriminate_inject H0.
-  Defined.
+    constructor; unfold iAlgebra, WF_invertClos_P.
+    inversion 1; subst; simpl; split.
+    - apply (inject_i (subGF := Sub_WFV_VB_WFV)); econstructor; eauto.
+    - intros ? Heq; discriminate_inject Heq.
+  Qed.
 
   (* ============================================== *)
   (* EQUIVALENCE OF BOOLEAN EXPRESSIONS             *)
@@ -86,7 +71,7 @@ Section PLambda_Bool.
     C (mk_eqv_i _ _ _ gamma gamma' el el') ->
     Bool_eqv A B C (mk_eqv_i _ _ _ gamma gamma' (cond _ i t el) (cond _ i' t' el')).
 
-  Lemma Bool_eqv_impl_NP_eqv : forall A B C i,
+  Lemma Bool_eqv_impl_NP_eqv A B C i :
     Bool_eqv A B C i -> NP_Functor_eqv E Bool A B C i.
   Proof.
     intros; destruct H.
@@ -98,7 +83,6 @@ Section PLambda_Bool.
       (np := fun D => If D); auto.
     simpl; intros; dependent destruction p; auto.
     simpl; congruence.
-  Defined.
-
+  Qed.
 
 End PLambda_Bool.
