CaseStudy/MiniML.v
@@ -1,7 +1,5 @@
-Require Import String.
-Require Import GDTC.Polynomial.
-Require Import GDTC.Containers.
-Require Import GDTC.Functors.
+Require Import Coq.Strings.String.
+Require Import GDTC.
 Require Import CaseStudy.Names.
 Require Import CaseStudy.PNames.
 Require Import CaseStudy.Arith.
@@ -20,10 +18,6 @@ Section MiniML.
 
   Global Instance Container_D : Container D :=
     PolynomialContainer D.
-
-  Global Instance SPF_D : SPF D.
-    eauto with typeclass_instances.
-  Defined.
 
   Definition E (A : Set) := Arith :+: (Lambda D A) :+: Bool :+: (Fix_ D A) :+: (NatCase A).
 
@@ -48,72 +42,10 @@ Section MiniML.
     eauto 150 with typeclass_instances.
   Defined.
 
-  (* Global Instance eq_DType_eq_D : *)
-  (*   PAlgebra eq_DType_eqName (sig (UP'_P (eq_DType_eq_P D))) D. *)
-  (* Proof. *)
-  (*   unfold D. *)
-  (*   eauto 20 with typeclass_instances. *)
-  (* Defined. *)
-
-  Definition Eqv (A B : Set) :=
-    (NP_Functor_eqv E Arith A B) ::+:: (NP_Functor_eqv E Bool A B) ::+::
-    (Lambda_eqv D E A B) ::+:: (Fix_eqv D E A B) ::+:: (NatCase_eqv E A B).
-
-  Definition WFV := (WFValue_Clos D E V Eqv (typeof _ _)) ::+::
-    (WFValue_Bot D V) ::+:: (WFValue_VI D V) ::+:: (WFValue_VB D V).
-
-  Global Instance Container_WFV : IContainer WFV.
-    eauto with typeclass_instances.
-  Defined.
-
   Definition SV := (SubValue_refl V) ::+:: (SubValue_Bot V) ::+:: (SubValue_Clos E V).
 
   Global Instance Container_SV : IContainer SV.
     eauto with typeclass_instances.
-  Defined.
-
-  Global Instance SV_invertVI_SV :
-    iPAlgebra SV_invertVI_Name (SV_invertVI_P V) SV.
-    repeat apply iPAlgebra_Plus; eauto 150 with typeclass_instances.
-    constructor.
-    unfold iAlgebra.
-    unfold SV_invertVI_P.
-    intros i H n H0.
-    inversion H; subst.
-    elimtype False; apply (inject_discriminate _ _ _ H0).
-  Defined.
-
-  Global Instance SV_invertVI'_SV :
-    iPAlgebra SV_invertVI'_Name (SV_invertVI'_P V) SV.
-    repeat apply iPAlgebra_Plus; eauto 150 with typeclass_instances.
-    constructor.
-    unfold iAlgebra.
-    unfold SV_invertVI'_P.
-    intros i H n H0.
-    inversion H; subst.
-    elimtype False; apply (inject_discriminate _ _ _ H0).
-  Defined.
-
-  Global Instance SV_invertVB_SV :
-    iPAlgebra SV_invertVB_Name (SV_invertVB_P V) SV.
-    repeat apply iPAlgebra_Plus; eauto 150 with typeclass_instances.
-    constructor.
-    unfold iAlgebra.
-    unfold SV_invertVB_P.
-    intros i H n H0.
-    inversion H; subst.
-    elimtype False; apply (inject_discriminate _ _ _ H0).
-  Defined.
-
-  Global Instance SV_invertVB'_SV :
-    iPAlgebra SV_invertVB'_Name (SV_invertVB'_P V) SV.
-    repeat apply iPAlgebra_Plus; eauto 150 with typeclass_instances.
-    constructor.
-    unfold iAlgebra.
-    unfold SV_invertVB'_P.
-    intros i H n H0.
-    inversion H; subst.
-    elimtype False; apply (inject_discriminate _ _ _ H0).
   Defined.
 
   Global Instance EV_Alg :
@@ -126,7 +58,7 @@ Section MiniML.
       eauto 200 with typeclass_instances.
     - generalize (@NatCase_eval_continuous_Exp E _ _ _ _).
       eauto 200 with typeclass_instances.
-  Defined.
+  Qed.
 
   Lemma eval_continuous : forall m,
     forall (e : Exp E nat) (gamma gamma' : Env _),
@@ -138,41 +70,36 @@ Section MiniML.
 
   Eval compute in ("Continuity of Evaluation Proven for MiniML!").
 
-  (* Global Instance Bool_sound P_bind P pb typeof_rec eval_rec : *)
-  (*   PAlgebra eval_Soundness_alg_Name *)
-  (*   (sig (UP'_P2 (eval_alg_Soundness_P D V (E nat) WFV P_bind P *)
-  (*     (E (typeofR D)) (Fun_E (typeofR D)) pb typeof_rec *)
-  (*     eval_rec f_algebra f_algebra))) Bool. *)
-  (* Proof. *)
-  (*   eauto 250 with typeclass_instances. *)
-  (* Defined. *)
+  Definition Eqv (A B : Set) :=
+    (NP_Functor_eqv E Arith A B) ::+:: (NP_Functor_eqv E Bool A B) ::+::
+    (Lambda_eqv D E A B) ::+:: (Fix_eqv D E A B) ::+:: (NatCase_eqv E A B).
+  Global Instance Container_Eqv : forall (A B : Set), IContainer (Eqv A B).
+    eauto with typeclass_instances.
+  Defined.
 
-  Instance Eval_Soundness_alg :
-    forall
-      eval_rec : Names.Exp (E nat) -> evalR V,
-      iPAlgebra soundness_XName
-                (soundness_X'_P D V E Eqv WFV
-                                (typeof D (E (typeofR D))) eval_rec
-                                (f_algebra TypeofName) (f_algebra EvalName))
-                (Eqv (typeofR D) nat).
-  Proof.
-    assert (WF_FAlgebra_eval_Lambda :
-              WF_FAlgebra EvalName (Names.Exp (E nat)) (evalR V)
-                (Lambda D nat) (E nat) (MAlgebra_eval_Lambda D E V) V_eval).
-    eauto 500 with typeclass_instances.
-    intros.
-    repeat apply iPAlgebra_Plus.
-    - apply Lift_soundness_X_alg.
-      + eauto with typeclass_instances.
-      + apply eqv_eval_Soundness; eauto 250 with typeclass_instances.
-    - apply Lift_soundness_X_alg.
-      + eauto with typeclass_instances.
-      + apply eqv_eval_Soundness; eauto 250 with typeclass_instances.
-    - eapply Lambda_eqv_eval_soundness_alg; eauto 250 with typeclass_instances.
-    - eapply Fix_Soundness; eauto 250 with typeclass_instances.
-    - apply Lift_soundness_X_alg.
-      + eauto with typeclass_instances.
-      + eapply NatCase_eval_Soundness; eauto 250 with typeclass_instances.
+  Definition WFV := (WFValue_Clos D E V Eqv (typeof _ _)) ::+::
+    (WFValue_Bot D V) ::+:: (WFValue_VI D V) ::+:: (WFValue_VB D V).
+
+  Global Instance Container_WFV : IContainer WFV.
+    eauto with typeclass_instances.
+  Defined.
+
+  Instance Eval_Soundness_alg (eval_rec : Exp E nat -> evalR V) :
+    iPAlgebra soundness_XName
+              (soundness_X'_P D V E Eqv WFV
+                              (typeof D (E (typeofR D))) eval_rec
+                              (f_algebra TypeofName) (f_algebra EvalName))
+              (Eqv (typeofR D) nat).
+  Proof with eauto 200 with typeclass_instances.
+    repeat apply iPAlgebra_Plus...
+    - apply Lift_soundness_X_alg...
+      apply eqv_eval_Soundness...
+    - apply Lift_soundness_X_alg...
+      apply eqv_eval_Soundness...
+    - eapply Lambda_eqv_eval_soundness_alg...
+    - eapply Fix_Soundness...
+    - apply Lift_soundness_X_alg...
+      eapply NatCase_eval_Soundness...
   Qed.
 
   Theorem soundness : forall n gamma gamma' gamma'' e' e'',
@@ -185,10 +112,6 @@ Section MiniML.
     typeof D (E _) e' = Some T -> WFValueC _ _ WFV (beval _ _ n e'' gamma'') T.
   Proof.
     eapply soundness_X; eauto 800 with typeclass_instances.
-    repeat apply iPAlgebra_Plus; eauto 800 with typeclass_instances.
-    apply (@WFV_Value_continuous_Clos D _ _ _ _ E _ _ _ V _ _ _ _ Eqv _ _ WFV _ _
-                                      (typeof D (E (typeofR D))));
-    eauto 800 with typeclass_instances.
   Qed.
 
   Eval compute in ("Type Soundness for MiniML Proven!").
