CaseStudy/test_ABL.v
@@ -1,7 +1,5 @@
-Require Import String.
-Require Import GDTC.Polynomial.
-Require Import GDTC.Containers.
-Require Import GDTC.Functors.
+Require Import Coq.Strings.String.
+Require Import GDTC.
 Require Import CaseStudy.Names.
 Require Import CaseStudy.PNames.
 Require Import CaseStudy.Arith.
@@ -18,10 +16,6 @@ Section Type_Test_Section.
 
   Global Instance Container_D : Container D :=
     PolynomialContainer D.
-
-  Global Instance SPF_D : SPF D.
-    eauto with typeclass_instances.
-  Defined.
 
   Definition tex2 : DType D := tnat _.
   Definition tex3 : DType D := tarrow _ tex2 tex2. (* Nat -> Nat *)
@@ -45,13 +39,13 @@ End Type_Test_Section.
 
 Section Test_Section.
 
-  Definition E (A : Set) := Arith :+: (Lambda D A) :+: Bool.
+  Definition E (A: Set) := Arith :+: (Lambda D A) :+: Bool.
 
   Global Instance Container_E : forall (A : Set), Container (E A).
     eauto with typeclass_instances.
   Defined.
 
-  Definition ex_3 A : Names.Exp (E A) := (lit _ 1). (* ex_3 := 1 *)
+  Definition ex_3 A : Exp E A := (lit _ 1). (* ex_3 := 1 *)
 
   (* Definition ex_1 (A : Set) t1 t2 : Names.Exp (E A) := (* ex_1 := (\x : t1. x) (\y : t2 . y) *) *)
   (*   app D E (lam D E t1 (fun e : A => var D E e)) (lam D E t2 (fun e : A => var D E e)). *)
@@ -113,20 +107,6 @@ Section Test_Section.
   (* Eval compute in ("Evaluating '\x. x'"). *)
   (* Eval compute in (ValuePrint V (proj1_sig (beval V _ 5 (ex_id _) nil))). *)
 
-  Definition Eqv (A B : Set) :=
-    (NP_Functor_eqv E Arith A B) ::+:: (NP_Functor_eqv E Bool A B) ::+::
-    (Lambda_eqv D E A B).
-
-  Global Instance Container_Eqv : forall (A B : Set), IContainer (Eqv A B).
-    eauto with typeclass_instances.
-  Defined.
-
-  Definition WFV := (WFValue_Clos D E V Eqv (typeof _ _)) ::+:: (WFValue_Bot D V) ::+::
-    (WFValue_VI D V) ::+:: (WFValue_VB D V).
-
-  Global Instance Container_WFV : IContainer WFV.
-    eauto with typeclass_instances.
-  Defined.
 
   Definition SV := (SubValue_refl V) ::+:: (SubValue_Bot V) ::+:: (SubValue_Clos E V).
 
@@ -134,55 +114,11 @@ Section Test_Section.
     eauto with typeclass_instances.
   Defined.
 
-  Global Instance SV_invertVI_SV :
-    iPAlgebra SV_invertVI_Name (SV_invertVI_P V) SV.
-    repeat apply iPAlgebra_Plus; eauto 150 with typeclass_instances.
-    constructor.
-    unfold iAlgebra.
-    unfold SV_invertVI_P.
-    intros i H n H0.
-    inversion H; subst.
-    elimtype False; apply (inject_discriminate _ _ _ H0).
-  Defined.
-
-  Global Instance SV_invertVI'_SV :
-    iPAlgebra SV_invertVI'_Name (SV_invertVI'_P V) SV.
-    repeat apply iPAlgebra_Plus; eauto 150 with typeclass_instances.
-    constructor.
-    unfold iAlgebra.
-    unfold SV_invertVI'_P.
-    intros i H n H0.
-    inversion H; subst.
-    elimtype False; apply (inject_discriminate _ _ _ H0).
-  Defined.
-
-  Global Instance SV_invertVB_SV :
-    iPAlgebra SV_invertVB_Name (SV_invertVB_P V) SV.
-    repeat apply iPAlgebra_Plus; eauto 150 with typeclass_instances.
-    constructor.
-    unfold iAlgebra.
-    unfold SV_invertVB_P.
-    intros i H n H0.
-    inversion H; subst.
-    elimtype False; apply (inject_discriminate _ _ _ H0).
-  Defined.
-
-  Global Instance SV_invertVB'_SV :
-    iPAlgebra SV_invertVB'_Name (SV_invertVB'_P V) SV.
-    repeat apply iPAlgebra_Plus; eauto 150 with typeclass_instances.
-    constructor.
-    unfold iAlgebra.
-    unfold SV_invertVB'_P.
-    intros i H n H0.
-    inversion H; subst.
-    elimtype False; apply (inject_discriminate _ _ _ H0).
-  Defined.
-
   Global Instance EV_Alg :
     FPAlgebra (eval_continuous_Exp_P V (E nat) SV) (inject (E nat) (E nat)).
   Proof.
     repeat apply FPAlgebra_Plus_cont_inject; eauto 200 with typeclass_instances.
-    - generalize (@Lambda_eval_continuous_Exp D _ _ _ E _ _ _ _).
+    - pose proof (Lambda_eval_continuous_Exp D E).
       eauto 200 with typeclass_instances.
   Qed.
 
@@ -196,43 +132,33 @@ Section Test_Section.
 
   Eval compute in ("Continuity of Evaluation Proven!").
 
-  Hint Extern 0 (id _) => unfold id; eauto with typeclass_instaces : typeclass_instances.
-
- (*
-  Global Instance Bool_sound P_bind P pb typeof_rec eval_rec :
-    PAlgebra eval_Soundness_alg_Name
-    (sig (UP'_P2 (eval_alg_Soundness_P D V (E nat) WFV P_bind P
-      (E (typeofR D)) (Fun_E (typeofR D)) pb typeof_rec
-      eval_rec f_algebra f_algebra))) Bool.
-  eauto 250 with typeclass_instances.
+  Definition Eqv (A B : Set) :=
+    (NP_Functor_eqv E Arith A B) ::+:: (NP_Functor_eqv E Bool A B) ::+::
+    (Lambda_eqv D E A B).
+  Global Instance Container_Eqv : forall (A B : Set), IContainer (Eqv A B).
+    eauto with typeclass_instances.
   Defined.
-*)
 
-  Instance Eval_Soundness_alg :
-    forall
-      eval_rec : Names.Exp (E nat) -> evalR V,
-      iPAlgebra soundness_XName
-                (soundness_X'_P D V E Eqv WFV
-                                (typeof D (E (typeofR D))) eval_rec
-                                (f_algebra TypeofName) (f_algebra EvalName))
-                (Eqv (typeofR D) nat).
-  Proof.
-    assert (WF_FAlgebra_eval_Lambda :
-              WF_FAlgebra EvalName (Names.Exp (E nat)) (evalR V)
-                (Lambda D nat) (E nat) (MAlgebra_eval_Lambda D E V) V_eval).
-    eauto 500 with typeclass_instances.
-    intros.
-    repeat apply iPAlgebra_Plus.
-    apply Lift_soundness_X_alg.
+  Definition WFV := (WFValue_Clos D E V Eqv (typeof _ _)) ::+:: (WFValue_Bot D V) ::+::
+    (WFValue_VI D V) ::+:: (WFValue_VB D V).
+
+  Global Instance Container_WFV : IContainer WFV.
     eauto with typeclass_instances.
-    apply eqv_eval_Soundness;
-    eauto 250 with typeclass_instances.
-    apply Lift_soundness_X_alg.
-    eauto with typeclass_instances.
-    apply eqv_eval_Soundness;
-    eauto 250 with typeclass_instances.
-    apply (@Lambda_eqv_eval_soundness_alg D _ _ _ _ _ E _ _ _ _ V _ _ _ _ _ _ _ V_eval WF_FAlgebra_eval_Lambda _ _ Eqv _ _ _ _ WFV _ _ (typeof D (E (typeofR D)))); eauto with typeclass_instances.
-    eauto 250 with typeclass_instances.
+  Defined.
+
+  Instance Eval_Soundness_alg (eval_rec : Exp E nat -> evalR V) :
+    iPAlgebra soundness_XName
+              (soundness_X'_P D V E Eqv WFV
+                              (typeof D (E (typeofR D))) eval_rec
+                              (f_algebra TypeofName) (f_algebra EvalName))
+              (Eqv (typeofR D) nat).
+  Proof with eauto 200 with typeclass_instances.
+    repeat apply iPAlgebra_Plus...
+    - apply Lift_soundness_X_alg...
+      apply eqv_eval_Soundness...
+    - apply Lift_soundness_X_alg...
+      apply eqv_eval_Soundness...
+    - pose proof (Lambda_eqv_eval_soundness_alg D E)...
   Qed.
 
   Theorem soundness : forall n gamma gamma' gamma'' e' e'',
@@ -244,7 +170,7 @@ Section Test_Section.
     (WF_gamma'' : WF_Environment _ _ WFV gamma'' gamma) T,
     typeof D (E _) e' = Some T -> WFValueC _ _ WFV (beval _ _ n e'' gamma'') T.
   Proof.
-    eapply soundness_X; eauto 800 with typeclass_instances.
+    eapply soundness_X; eauto 350 with typeclass_instances.
   Qed.
 
   Eval compute in ("Type Soundness for Arith :+: Lambda :+: Boolean Proven!").
