GDTC.v
@@ -1,0 +1,5 @@
+Require Export GDTC.Containers.
+Require Export GDTC.FJ_tactics.
+Require Export GDTC.Functors.
+Require Export GDTC.Polynomial.
+Require Export GDTC.Equality.
