GDTC/Functors.v
@@ -1,6 +1,28 @@
-Load FJ_tactics.
-Require Import List.
-Require Import FunctionalExtensionality.
+Require Import Coq.Lists.List.
+Require Import Coq.Logic.FunctionalExtensionality.
+
+Require Import FJ_tactics.
+
+Section Sums.
+
+  Definition fold_sum {A B : Type} {C : sum A B -> Type}
+             (f : forall (a : A), C (inl _ a))
+             (g : forall (b : B), C (inr _ b))
+             (x : A + B) : C x :=
+    match x with
+    | inl y => f y
+    | inr y => g y
+    end.
+
+  Definition fold_sum' {A B : Type} {C : Type}
+    (f : A -> C) (g : B -> C) (x : A + B) : C :=
+    @fold_sum A B (fun _ => C) f g x.
+
+  Definition map_sum {A B C D : Type} (f : A -> C) (g : B -> D)
+    (x : A + B) : C + D :=
+    fold_sum (fun x => inl _ (f x)) (fun x => inr _ (g x)) x.
+
+End Sums.
 
 Section Functors.
   Class Functor (F : Set -> Set) :=
