GDTC/Polynomial.v
@@ -1,11 +1,11 @@
 Require Import Coq.Bool.Bool.
+Require Import Coq.Lists.List.
 Require Import Coq.Logic.Eqdep.
+Require Import Coq.Logic.FunctionalExtensionality.
 Require Import Coq.Program.Equality.
 
 Require Import Containers.
 Require Import Functors.
-Require Import List.
-Require Import FunctionalExtensionality.
 
 Inductive Code : Set :=
 | U : Code
@@ -246,116 +246,116 @@ Section Fold2.
 
 End Fold2.
 
-Section Equality.
+(* Section Equality. *)
 
-  Class Eq (A : Set) :=
-    { eq                     :  A -> A -> bool;
-      eq_propositional_true  : forall (x y : A), eq x y = true  -> x = y;
-      eq_propositional_false : forall (x y : A), eq x y = false -> x <> y
-    }.
+(*   Class Eq (A : Set) := *)
+(*     { eq                     :  A -> A -> bool; *)
+(*       eq_propositional_true  : forall (x y : A), eq x y = true  -> x = y; *)
+(*       eq_propositional_false : forall (x y : A), eq x y = false -> x <> y *)
+(*     }. *)
 
-  Variable c : Code.
+(*   Variable c : Code. *)
 
-  Definition EQA := FixP c -> bool.
-  Definition EQB (d : Code) := ExtP (FixP c) d -> bool.
+(*   Definition EQA := FixP c -> bool. *)
+(*   Definition EQB (d : Code) := ExtP (FixP c) d -> bool. *)
 
-  (*
-  Fixpoint eqalg (d : Code) (x : ExtP EQA d) : EQB d.
-  Proof.
-    destruct x; intro y.
-    apply true.
-    inversion y.
-    apply (e H).
-    inversion y; subst.
-    apply (eqalg _ _ H0).
-    unfold
-  *)
+(*   (* *)
+(*   Fixpoint eqalg (d : Code) (x : ExtP EQA d) : EQB d. *)
+(*   Proof. *)
+(*     destruct x; intro y. *)
+(*     apply true. *)
+(*     inversion y. *)
+(*     apply (e H). *)
+(*     inversion y; subst. *)
+(*     apply (eqalg _ _ H0). *)
+(*     unfold *)
+(*   *) *)
 
-  Definition eqf (eq : EQB c) : EQA :=
-    fun x => match x with
-               | fixp e => eq e
-             end.
-  Definition equ (x : ExtP (FixP c) U) : bool := true.
-  Definition eqi (f : EQA) : EQB I :=
-    fun x => match x with
-               | ei x => f x
-               | _     => false
-             end.
-  Definition eql (c1 c2 : Code) (eq : EQB c1) : EQB (C c1 c2).
-    intro x; inversion x; subst.
-    apply (eq H0).
-    apply false.
-  Defined.
-  Definition eqr (c1 c2 : Code) (eq : EQB c2) : EQB (C c1 c2).
-    intro x; inversion x; subst.
-    apply false.
-    apply (eq H0).
-  Defined.
-  Definition eqp (c1 c2 : Code) (eq1 : EQB c1) (eq2 : EQB c2) : EQB (P c1 c2).
-    intro x; inversion x; subst.
-    apply (andb (eq1 H1) (eq2 H2)).
-  Defined.
+(*   Definition eqf (eq : EQB c) : EQA := *)
+(*     fun x => match x with *)
+(*                | fixp e => eq e *)
+(*              end. *)
+(*   Definition equ (x : ExtP (FixP c) U) : bool := true. *)
+(*   Definition eqi (f : EQA) : EQB I := *)
+(*     fun x => match x with *)
+(*                | ei x => f x *)
+(*                | _     => false *)
+(*              end. *)
+(*   Definition eql (c1 c2 : Code) (eq : EQB c1) : EQB (C c1 c2). *)
+(*     intro x; inversion x; subst. *)
+(*     apply (eq H0). *)
+(*     apply false. *)
+(*   Defined. *)
+(*   Definition eqr (c1 c2 : Code) (eq : EQB c2) : EQB (C c1 c2). *)
+(*     intro x; inversion x; subst. *)
+(*     apply false. *)
+(*     apply (eq H0). *)
+(*   Defined. *)
+(*   Definition eqp (c1 c2 : Code) (eq1 : EQB c1) (eq2 : EQB c2) : EQB (P c1 c2). *)
+(*     intro x; inversion x; subst. *)
+(*     apply (andb (eq1 H1) (eq2 H2)). *)
+(*   Defined. *)
 
-  Definition eqfix : FixP c -> FixP c -> bool :=
-    fixpfold2 c EQA EQB eqf equ eqi eql eqr eqp.
-  Definition eqext : forall d, ExtP (FixP c) d -> ExtP (FixP c) d -> bool :=
-    extpfold2 c EQA EQB eqf equ eqi eql eqr eqp.
+(*   Definition eqfix : FixP c -> FixP c -> bool := *)
+(*     fixpfold2 c EQA EQB eqf equ eqi eql eqr eqp. *)
+(*   Definition eqext : forall d, ExtP (FixP c) d -> ExtP (FixP c) d -> bool := *)
+(*     extpfold2 c EQA EQB eqf equ eqi eql eqr eqp. *)
 
-  Lemma eqfix_propositional_true :
-    forall u v, eqfix u v = true -> u = v.
-  Proof.
-    apply (fixp_ind c
-            (fun u   => forall v, eqfix u v = true -> u = v)
-            (fun d u => forall v, eqext d u v = true -> u = v));
-      intros;
-      dependent destruction v;
-      try (f_equal; apply (H _ H0));
-      try discriminate.
-    (* ep *)
-    unfold eqext in H1.
-    unfold extpfold2 in H1.
-    simpl in H1.
-    apply andb_true_iff in H1.
-    destruct H1.
-    f_equal.
-    apply (H _ H1).
-    apply (H0 _ H2).
-  Qed.
+(*   Lemma eqfix_propositional_true : *)
+(*     forall u v, eqfix u v = true -> u = v. *)
+(*   Proof. *)
+(*     apply (fixp_ind c *)
+(*             (fun u   => forall v, eqfix u v = true -> u = v) *)
+(*             (fun d u => forall v, eqext d u v = true -> u = v)); *)
+(*       intros; *)
+(*       dependent destruction v; *)
+(*       try (f_equal; apply (H _ H0)); *)
+(*       try discriminate. *)
+(*     (* ep *) *)
+(*     unfold eqext in H1. *)
+(*     unfold extpfold2 in H1. *)
+(*     simpl in H1. *)
+(*     apply andb_true_iff in H1. *)
+(*     destruct H1. *)
+(*     f_equal. *)
+(*     apply (H _ H1). *)
+(*     apply (H0 _ H2). *)
+(*   Qed. *)
 
-  Lemma eqfix_propositional_false :
-    forall u v, eqfix u v = false -> u <> v.
-  Proof.
-    apply (fixp_ind c
-            (fun u   => forall v, eqfix u v = false -> u <> v)
-            (fun d u => forall v, eqext d u v = false -> u <> v));
-      intros;
-      dependent destruction v;
-      try discriminate;
-      intro Heq; inversion Heq; subst.
-    apply (H e); auto.
-    apply (H f); auto.
-    apply inj_pairT2 in H2.
-    apply (H _ H0); auto.
-    apply inj_pairT2 in H2.
-    apply (H _ H0); auto.
-    apply inj_pairT2 in H3.
-    apply inj_pairT2 in H4.
-    subst.
-    unfold eqext in H1.
-    unfold extpfold2 in H1.
-    simpl in H1.
-    apply andb_false_iff in H1.
-    destruct H1.
-    apply (H _ H1); auto.
-    apply (H0 _ H1) ; auto.
-  Qed.
+(*   Lemma eqfix_propositional_false : *)
+(*     forall u v, eqfix u v = false -> u <> v. *)
+(*   Proof. *)
+(*     apply (fixp_ind c *)
+(*             (fun u   => forall v, eqfix u v = false -> u <> v) *)
+(*             (fun d u => forall v, eqext d u v = false -> u <> v)); *)
+(*       intros; *)
+(*       dependent destruction v; *)
+(*       try discriminate; *)
+(*       intro Heq; inversion Heq; subst. *)
+(*     apply (H e); auto. *)
+(*     apply (H f); auto. *)
+(*     apply inj_pairT2 in H2. *)
+(*     apply (H _ H0); auto. *)
+(*     apply inj_pairT2 in H2. *)
+(*     apply (H _ H0); auto. *)
+(*     apply inj_pairT2 in H3. *)
+(*     apply inj_pairT2 in H4. *)
+(*     subst. *)
+(*     unfold eqext in H1. *)
+(*     unfold extpfold2 in H1. *)
+(*     simpl in H1. *)
+(*     apply andb_false_iff in H1. *)
+(*     destruct H1. *)
+(*     apply (H _ H1); auto. *)
+(*     apply (H0 _ H1) ; auto. *)
+(*   Qed. *)
 
-  Global Instance Eq_FixP : Eq (FixP c) :=
-    {| eq := eqfix;
-       eq_propositional_true := eqfix_propositional_true;
-       eq_propositional_false := eqfix_propositional_false |}.
+(*   Global Instance Eq_FixP : Eq (FixP c) := *)
+(*     {| eq := eqfix; *)
+(*        eq_propositional_true := eqfix_propositional_true; *)
+(*        eq_propositional_false := eqfix_propositional_false |}. *)
 
-End Equality.
+(* End Equality. *)
 
 Section Container.
 
@@ -582,21 +582,6 @@ Section Container.
     apply fromPolynomial_toPolynomial_inverse.
   Defined.
 
-  Global Instance Eq_Fix (F : Set -> Set) {poly_F : Polynomial F} :
-    Eq (Fix F) := {| eq := fun x y => eq (toFixP _ x) (toFixP _ y) |}.
-  Proof.
-    intros; simpl.
-    apply eq_propositional_true in H.
-    apply f_equal with (f := fromFixP PCode) in H.
-    repeat rewrite fromFixP_toFixP_inverse in H.
-    auto.
-    intros.
-    apply eq_propositional_false in H.
-    intro.
-    apply H.
-    f_equal.
-    auto.
-  Defined.
 
   Global Instance WF_Functor_plus_poly_inl
     {F G H : Set -> Set}
@@ -630,37 +615,37 @@ Section Container.
     reflexivity.
   Defined.
 
-  Global Instance WF_Functor_plus_poly_inl'
-    {F G H : Set -> Set}
-    {Cont_F : Polynomial F}
-    {Cont_G : Polynomial G}
-    {Fun_H : Functor H}
-    {sub_FG_H : (F :+: G) :<: H}
-    {WF_Fun_FG_H : WF_Functor _ _ sub_FG_H (Fun_F := ContainerFunctor (F :+: G))}
-    :
-    WF_Functor _ _ (Sub_Functor_inl' sub_FG_H).
-  Proof.
-    constructor; intros; simpl.
-    rewrite wf_functor; simpl.
-    destruct (fromPolynomial A PCode (pfrom fa)).
-    reflexivity.
-  Defined.
+  (* Global Instance WF_Functor_plus_poly_inl' *)
+  (*   {F G H : Set -> Set} *)
+  (*   {Cont_F : Polynomial F} *)
+  (*   {Cont_G : Polynomial G} *)
+  (*   {Fun_H : Functor H} *)
+  (*   {sub_FG_H : (F :+: G) :<: H} *)
+  (*   {WF_Fun_FG_H : WF_Functor _ _ sub_FG_H (Fun_F := ContainerFunctor (F :+: G))} *)
+  (*   : *)
+  (*   WF_Functor _ _ (Sub_Functor_inl' sub_FG_H). *)
+  (* Proof. *)
+  (*   constructor; intros; simpl. *)
+  (*   rewrite wf_functor; simpl. *)
+  (*   destruct (fromPolynomial A PCode (pfrom fa)). *)
+  (*   reflexivity. *)
+  (* Defined. *)
 
-  Global Instance WF_Functor_plus_cont_inr'
-    {F G H : Set -> Set}
-    {Cont_F : Container F}
-    {Cont_G : Container G}
-    {Fun_H : Functor H}
-    {sub_FG_H : (F :+: G) :<: H}
-    {WF_Fun_FG_H : WF_Functor _ _ sub_FG_H (Fun_F := ContainerFunctor (F :+: G))}
-    :
-    WF_Functor _ _ (Sub_Functor_inr' sub_FG_H).
-  Proof.
-    constructor; intros; simpl.
-    rewrite wf_functor; simpl.
-    destruct (from fa).
-    reflexivity.
-  Defined.
+  (* Global Instance WF_Functor_plus_cont_inr' *)
+  (*   {F G H : Set -> Set} *)
+  (*   {Cont_F : Container F} *)
+  (*   {Cont_G : Container G} *)
+  (*   {Fun_H : Functor H} *)
+  (*   {sub_FG_H : (F :+: G) :<: H} *)
+  (*   {WF_Fun_FG_H : WF_Functor _ _ sub_FG_H (Fun_F := ContainerFunctor (F :+: G))} *)
+  (*   : *)
+  (*   WF_Functor _ _ (Sub_Functor_inr' sub_FG_H). *)
+  (* Proof. *)
+  (*   constructor; intros; simpl. *)
+  (*   rewrite wf_functor; simpl. *)
+  (*   destruct (from fa). *)
+  (*   reflexivity. *)
+  (* Defined. *)
 
 End Container.
 
